Abstracted the ExecutionModel over the language

fairness/heap_lang/heap_lang_defs.v
@@ -2,47 +2,17 @@ From iris.base_logic Require Export gen_heap.
 From trillium.program_logic Require Export weakestpre.
 (* From trillium.fairness Require Export resources fuel. *)
 From trillium.fairness.heap_lang Require Export lang.
-
-Class ExecutionModel (M: Model) := {
-
-    (* TODO: how to express that these two are typeclasses themselves? *)
-    em_preGS: gFunctors -> Set;
-    em_GS: gFunctors -> Set;
-    em_Σ: gFunctors;
-    em_Σ_subG: forall Σ, subG em_Σ Σ -> em_preGS Σ;        
-
-    (* em_valid_state_evolution_fairness: execution_trace heap_lang -> auxiliary_trace M -> Prop; *)
-    em_valid_evolution_step:
-    olocale heap_lang → cfg heap_lang → mstate M → mlabel M → mstate M → Prop;
-
-    (* em_fork_post {Σ} *)
-    em_thread_post {Σ} `{em_GS Σ}
-    : locale heap_lang ->
-      (* val -> *)
-      iProp Σ;
-    em_msi {Σ} `{em_GS Σ}: cfg heap_lang -> mstate M -> iProp Σ;
-    
-    em_init_resource {Σ: gFunctors} `{em_GS Σ}: mstate M → iProp Σ;
-    (* TODO: currently we assume that postconditions of all threads coincide *)
-    (* em_init_thread_post {Σ}: locale heap_lang -> val -> iProp Σ; *)
-    em_is_init_st: cfg heap_lang -> mstate M -> Prop;
-    
-    em_initialization Σ `{ePreGS: em_preGS Σ}: 
-    forall (s1: mstate M) (σ: cfg heap_lang)
-      (INIT_ST: em_is_init_st σ s1),
-      ⊢ (|==> ∃ eGS: em_GS Σ, @em_init_resource _ eGS s1 ∗ @em_msi _ eGS σ s1)
-}.
-
+From trillium.fairness Require Export execution_model.
 
 (* TODO: the missing fact of em_GS etc. being typeclasses
    hardens automatic resolution of their instances *)
-Class heapGpreS Σ `(EM: ExecutionModel) := HeapPreG {
+Class heapGpreS Σ `(EM: ExecutionModel heap_lang M) := HeapPreG {
   heapGpreS_inv :> invGpreS Σ;
   heapGpreS_gen_heap :> gen_heapGpreS loc val Σ;
   heapGpreS_em :> em_preGS Σ;
 }.
 
-Class heapGS Σ `(EM: ExecutionModel) := HeapG {
+Class heapGS Σ `(EM: ExecutionModel heap_lang M) := HeapG {
   heap_inG :> heapGpreS Σ EM;
 
   heap_invGS :> invGS_gen HasNoLc Σ;
@@ -51,11 +21,11 @@ Class heapGS Σ `(EM: ExecutionModel) := HeapG {
   heap_fairnessGS :> em_GS Σ;
 }.
 
-Definition heapΣ `(EM: ExecutionModel M) : gFunctors :=
+Definition heapΣ `(EM: ExecutionModel heap_lang M) : gFunctors :=
   #[ invΣ; gen_heapΣ loc val; em_Σ ].
 
 (* TODO: automatize *)
-Global Instance subG_heapPreG {Σ} `{EM: ExecutionModel M} :
+Global Instance subG_heapPreG {Σ} `{EM: ExecutionModel heap_lang M}:
   subG (heapΣ EM) Σ → heapGpreS Σ EM.
 Proof.
   intros. 
@@ -63,17 +33,7 @@ Proof.
   apply em_Σ_subG. solve_inG.
 Qed. 
 
-Definition em_valid_state_evolution_fairness `{EM: ExecutionModel M}
-  (extr : execution_trace heap_lang) (auxtr: auxiliary_trace M) :=
-  match extr, auxtr with
-  | (extr :tr[oζ]: σ), auxtr :tr[ℓ]: δ =>
-      (* labels_match (LM:=LM) oζ ℓ ∧ LM.(lm_ls_trans) (trace_last auxtr) ℓ δ ∧ *)
-      (* tids_smaller es δ *)
-      em_valid_evolution_step oζ σ (trace_last auxtr) ℓ δ
-  | _, _ => True
-  end.
-
-#[global] Instance heapG_irisG `{EM: ExecutionModel M} `{HGS: !heapGS Σ EM}:
+#[global] Instance heapG_irisG `{EM: ExecutionModel heap_lang M} `{HGS: !heapGS Σ EM}:
   irisG heap_lang M Σ := {
     state_interp extr auxtr :=
       (⌜em_valid_state_evolution_fairness extr auxtr⌝ ∗
@@ -82,9 +42,8 @@ Definition em_valid_state_evolution_fairness `{EM: ExecutionModel M}
     fork_post tid := fun _ => em_thread_post tid (em_GS0 := heap_fairnessGS);
 }.
 
-
 Section GeneralProperties.
-  Context `{EM: ExecutionModel M}. 
+  Context `{EM: ExecutionModel heap_lang M}. 
   Context `{HGS: @heapGS Σ _ EM}.
   Let eGS := heap_fairnessGS. 
 
@@ -174,115 +133,3 @@ Section GeneralProperties.
   Proof. apply locales_of_list_from_indexes. Qed.
 
 End GeneralProperties.
-
-(* (* TODO: uncomment this and remove duplicate code from fuel.v *) *)
-(* Section TracesMatch. *)
-(*   Context `{EM: ExecutionModel M}.  *)
-
-(*   (* TODO: Why do we need explicit [LM] here? *) *)
-
-(*   Definition valid_lift_fairness *)
-(*              (φ: execution_trace heap_lang -> auxiliary_trace M -> Prop) *)
-(*              (extr : execution_trace heap_lang) (auxtr : auxiliary_trace M) := *)
-(*     em_valid_state_evolution_fairness extr auxtr ∧ φ extr auxtr. *)
-
-(*   (* TODO: move*) *)
-(*   From trillium.fairness Require Export inftraces *)
-(*     fairness *)
-(*   . *)
-(*   Let auxtrace := trace (mstate M) (mlabel M). *)
-
-(*   Context (state_rel: cfg heap_lang -> mstate M -> Prop). *)
-(*   Context (lbl_rel: olocale heap_lang -> mlabel M -> Prop). *)
-(*   Hypothesis (LBL_REL_EM: forall oζ σ δ1 ℓ δ2, *)
-(*                  em_valid_evolution_step oζ σ δ1 ℓ δ2 -> *)
-(*                  lbl_rel oζ ℓ).  *)
-(*   Hypothesis (STEP_EM: forall oζ σ δ1 ℓ δ2, *)
-(*                  em_valid_evolution_step oζ σ δ1 ℓ δ2 -> *)
-(*                  mtrans δ1 ℓ δ2).  *)
-
-(*   Definition exaux_traces_match: *)
-(*     extrace heap_lang → auxtrace → Prop := *)
-(*     traces_match lbl_rel *)
-(*       state_rel *)
-(*       locale_step *)
-(*       (@mtrans M).  *)
-
-(*   (* TODO: Why do we need explicit [LM] here? *) *)
-(*   Lemma valid_inf_system_trace_implies_traces_match_strong *)
-(*         (φ : execution_trace heap_lang -> auxiliary_trace M -> Prop) *)
-(*         (ψ : _ → _ → Prop) *)
-(*         ex atr iex iatr progtr (auxtr : auxtrace): *)
-(*     (forall (ex: execution_trace heap_lang) (atr: auxiliary_trace M), *)
-(*         φ ex atr -> state_rel (trace_last ex) (trace_last atr)) -> *)
-(*     (forall (ex: execution_trace heap_lang) (atr: auxiliary_trace M), *)
-(*         φ ex atr -> em_valid_state_evolution_fairness ex atr) -> *)
-(*     (∀ extr auxtr, φ extr auxtr → ψ (trace_last extr) (trace_last auxtr)) → *)
-(*     exec_trace_match ex iex progtr -> *)
-(*     exec_trace_match atr iatr auxtr -> *)
-(*     valid_inf_system_trace φ ex atr iex iatr -> *)
-(*     traces_match lbl_rel *)
-(*                  (λ σ δ, state_rel σ δ ∧ ψ σ δ) *)
-(*                  locale_step *)
-(*                  (@mtrans M) progtr auxtr. *)
-(*   Proof.  *)
-(*     intros Hφ1 Hφ2 Hφψ. *)
-(*     revert ex atr iex iatr auxtr progtr. cofix IH. *)
-(*     intros ex atr iex iatr auxtr progtr Hem Ham Hval. *)
-(*     inversion Hval as [?? Hphi |ex' atr' c [? σ'] δ' iex' iatr' oζ ℓ Hphi [=] ? Hinf]; simplify_eq. *)
-(*     - inversion Hem; inversion Ham. econstructor; eauto. *)
-(*       pose proof (Hφ1 ex atr Hphi). *)
-(*       split; [by simplify_eq|]. simplify_eq. by apply Hφψ. *)
-(*     - inversion Hem; inversion Ham. subst. *)
-(*       pose proof (valid_inf_system_trace_inv _ _ _ _ _ Hinf) as Hphi'. *)
-(*       specialize (Hφ2 (ex :tr[ oζ ]: (l, σ')) (atr :tr[ ℓ ]: δ') Hphi') as STEP. *)
-(*       red in STEP.        *)
-(*       econstructor. *)
-(*       + eapply LBL_REL_EM; eauto.  *)
-(*       + eauto. *)
-(*       + match goal with *)
-(*         | [H: exec_trace_match _ iex' _ |- _] => inversion H; clear H; simplify_eq *)
-(*         end; done. *)
-(*       + match goal with *)
-(*         | [H: exec_trace_match _ iatr' _ |- _] => inversion H; clear H; simplify_eq *)
-(*         end; eapply STEP_EM; eauto.  *)
-(*       + eapply IH; eauto. *)
-(*   Qed. *)
-
-(*   (* TODO: Why do we need explicit [LM] here? *) *)
-(*   Lemma valid_inf_system_trace_implies_traces_match *)
-(*         (φ: execution_trace heap_lang -> auxiliary_trace M -> Prop) *)
-(*         ex atr iex iatr progtr (auxtr : auxtrace): *)
-(*     (forall (ex: execution_trace heap_lang) (atr: auxiliary_trace M), *)
-(*         φ ex atr -> state_rel (trace_last ex) (trace_last atr)) -> *)
-(*     (forall (ex: execution_trace heap_lang) (atr: auxiliary_trace M), *)
-(*         φ ex atr -> em_valid_state_evolution_fairness ex atr) -> *)
-(*     exec_trace_match ex iex progtr -> *)
-(*     exec_trace_match atr iatr auxtr -> *)
-(*     valid_inf_system_trace φ ex atr iex iatr -> *)
-(*     exaux_traces_match progtr auxtr. *)
-(*   Proof. *)
-(*     intros Hφ1 Hφ2. *)
-(*     revert ex atr iex iatr auxtr progtr. cofix IH. *)
-(*     intros ex atr iex iatr auxtr progtr Hem Ham Hval. *)
-(*     inversion Hval as [?? Hphi |ex' atr' c [? σ'] δ' iex' iatr' oζ ℓ Hphi [=] ? Hinf]; simplify_eq. *)
-(*     - inversion Hem; inversion Ham. econstructor; eauto. *)
-(*       pose proof (Hφ1 ex atr Hphi). *)
-(*       by simplify_eq. *)
-(*     - inversion Hem; inversion Ham. subst. *)
-(*       pose proof (valid_inf_system_trace_inv _ _ _ _ _ Hinf) as Hphi'. *)
-(*       specialize (Hφ2 (ex :tr[ oζ ]: (l, σ')) (atr :tr[ ℓ ]: δ') Hphi') as STEP. *)
-(*       red in STEP.        *)
-(*       econstructor. *)
-(*       + eauto. *)
-(*       + eauto. *)
-(*       + match goal with *)
-(*         | [H: exec_trace_match _ iex' _ |- _] => inversion H; clear H; simplify_eq *)
-(*         end; done. *)
-(*       + match goal with *)
-(*         | [H: exec_trace_match _ iatr' _ |- _] => inversion H; clear H; simplify_eq *)
-(*         end; eapply STEP_EM; eauto.  *)
-(*       + eapply IH; eauto. *)
-(*   Qed. *)
-
-(* End TracesMatch.  *)
