fairness/execution_model.v
@@ -1,0 +1,156 @@
+From stdpp Require Import fin_maps.
+From iris.proofmode Require Import tactics.
+From trillium Require Import language.
+From trillium.program_logic Require Import traces weakestpre.
+From trillium.fairness Require Import inftraces fairness. 
+
+Class ExecutionModel (Λ: language) (M: Model) := {
+
+    (* TODO: how to express that these two are typeclasses themselves? *)
+    em_preGS: gFunctors -> Set;
+    em_GS: gFunctors -> Set;
+    em_Σ: gFunctors;
+    em_Σ_subG: forall Σ, subG em_Σ Σ -> em_preGS Σ;
+
+    em_valid_evolution_step:
+    olocale Λ → cfg Λ → mstate M → mlabel M → mstate M → Prop;
+
+    (* em_fork_post {Σ} *)
+    em_thread_post {Σ} `{em_GS Σ}
+    : locale Λ ->
+      (* val -> *)
+      iProp Σ;
+    em_msi {Σ} `{em_GS Σ}: cfg Λ -> mstate M -> iProp Σ;
+    
+    em_init_resource {Σ: gFunctors} `{em_GS Σ}: mstate M → iProp Σ;
+    (* TODO: currently we assume that postconditions of all threads coincide *)
+    (* em_init_thread_post {Σ}: locale Λ -> val -> iProp Σ; *)
+    em_is_init_st: cfg Λ -> mstate M -> Prop;
+    
+    em_initialization Σ `{ePreGS: em_preGS Σ}: 
+    forall (s1: mstate M) (σ: cfg Λ)
+      (INIT_ST: em_is_init_st σ s1),
+      ⊢ (|==> ∃ eGS: em_GS Σ, @em_init_resource _ eGS s1 ∗ @em_msi _ eGS σ s1)
+}.
+
+Section EMDefinitions.
+  Context `{EM: ExecutionModel Λ M}. 
+
+  Definition em_valid_state_evolution_fairness
+    (extr : execution_trace Λ) (auxtr: auxiliary_trace M) :=
+    match extr, auxtr with
+    | (extr :tr[oζ]: σ), auxtr :tr[ℓ]: δ =>
+        (* labels_match (LM:=LM) oζ ℓ ∧ LM.(lm_ls_trans) (trace_last auxtr) ℓ δ ∧ *)
+        (* tids_smaller es δ *)
+      em_valid_evolution_step oζ σ (trace_last auxtr) ℓ δ
+    | _, _ => True
+    end.
+
+  (* TODO: where is that needed? *)
+  Definition valid_lift_fairness
+    (φ: execution_trace Λ -> auxiliary_trace M -> Prop)
+    (extr : execution_trace Λ) (auxtr : auxiliary_trace M) :=
+    em_valid_state_evolution_fairness extr auxtr ∧ φ extr auxtr.
+
+End EMDefinitions.
+
+
+(* Section TracesMatch. *)
+(*   Context `{EM: ExecutionModel Λ M}. *)
+
+(*   Let auxtrace := trace (mstate M) (mlabel M). *)
+
+(*   Context (state_rel: cfg Λ -> mstate M -> Prop). *)
+(*   Context (lbl_rel: olocale Λ -> mlabel M -> Prop). *)
+(*   Hypothesis (LBL_REL_EM: forall oζ σ δ1 ℓ δ2, *)
+(*                  em_valid_evolution_step oζ σ δ1 ℓ δ2 -> *)
+(*                  lbl_rel oζ ℓ). *)
+(*   Hypothesis (STEP_EM: forall oζ σ δ1 ℓ δ2, *)
+(*                  em_valid_evolution_step oζ σ δ1 ℓ δ2 -> *)
+(*                  mtrans δ1 ℓ δ2). *)
+
+(*   Definition exaux_traces_match: *)
+(*     extrace Λ → auxtrace → Prop := *)
+(*     traces_match lbl_rel *)
+(*       state_rel *)
+(*       locale_step *)
+(*       (@mtrans M). *)
+
+(*   (* TODO: Why do we need explicit [LM] here? *) *)
+(*   Lemma valid_inf_system_trace_implies_traces_match_strong *)
+(*         (φ : execution_trace Λ -> auxiliary_trace M -> Prop) *)
+(*         (ψ : _ → _ → Prop) *)
+(*         ex atr iex iatr progtr (auxtr : auxtrace): *)
+(*     (forall (ex: execution_trace Λ) (atr: auxiliary_trace M), *)
+(*         φ ex atr -> state_rel (trace_last ex) (trace_last atr)) -> *)
+(*     (forall (ex: execution_trace Λ) (atr: auxiliary_trace M), *)
+(*         φ ex atr -> em_valid_state_evolution_fairness ex atr) -> *)
+(*     (∀ extr auxtr, φ extr auxtr → ψ (trace_last extr) (trace_last auxtr)) → *)
+(*     exec_trace_match ex iex progtr -> *)
+(*     exec_trace_match atr iatr auxtr -> *)
+(*     valid_inf_system_trace φ ex atr iex iatr -> *)
+(*     traces_match lbl_rel *)
+(*                  (λ σ δ, state_rel σ δ ∧ ψ σ δ) *)
+(*                  locale_step *)
+(*                  (@mtrans M) progtr auxtr. *)
+(*   Proof. *)
+(*     intros Hφ1 Hφ2 Hφψ. *)
+(*     revert ex atr iex iatr auxtr progtr. cofix IH. *)
+(*     intros ex atr iex iatr auxtr progtr Hem Ham Hval. *)
+(*     inversion Hval as [?? Hphi |ex' atr' c [? σ'] δ' iex' iatr' oζ ℓ Hphi [=] ? Hinf]; simplify_eq. *)
+(*     - inversion Hem; inversion Ham. econstructor; eauto. *)
+(*       pose proof (Hφ1 ex atr Hphi). *)
+(*       split; [by simplify_eq|]. simplify_eq. by apply Hφψ. *)
+(*     - inversion Hem; inversion Ham. subst. *)
+(*       pose proof (valid_inf_system_trace_inv _ _ _ _ _ Hinf) as Hphi'. *)
+(*       specialize (Hφ2 (ex :tr[ oζ ]: (l, σ')) (atr :tr[ ℓ ]: δ') Hphi') as STEP. *)
+(*       red in STEP. *)
+(*       econstructor. *)
+(*       + eapply LBL_REL_EM; eauto. *)
+(*       + eauto. *)
+(*       + match goal with *)
+(*         | [H: exec_trace_match _ iex' _ |- _] => inversion H; clear H; simplify_eq *)
+(*         end; done. *)
+(*       + match goal with *)
+(*         | [H: exec_trace_match _ iatr' _ |- _] => inversion H; clear H; simplify_eq *)
+(*         end; eapply STEP_EM; eauto. *)
+(*       + eapply IH; eauto. *)
+(*   Qed. *)
+
+(*   (* TODO: Why do we need explicit [LM] here? *) *)
+(*   Lemma valid_inf_system_trace_implies_traces_match *)
+(*         (φ: execution_trace Λ -> auxiliary_trace M -> Prop) *)
+(*         ex atr iex iatr progtr (auxtr : auxtrace): *)
+(*     (forall (ex: execution_trace Λ) (atr: auxiliary_trace M), *)
+(*         φ ex atr -> state_rel (trace_last ex) (trace_last atr)) -> *)
+(*     (forall (ex: execution_trace Λ) (atr: auxiliary_trace M), *)
+(*         φ ex atr -> em_valid_state_evolution_fairness ex atr) -> *)
+(*     exec_trace_match ex iex progtr -> *)
+(*     exec_trace_match atr iatr auxtr -> *)
+(*     valid_inf_system_trace φ ex atr iex iatr -> *)
+(*     exaux_traces_match progtr auxtr. *)
+(*   Proof. *)
+(*     intros Hφ1 Hφ2. *)
+(*     revert ex atr iex iatr auxtr progtr. cofix IH. *)
+(*     intros ex atr iex iatr auxtr progtr Hem Ham Hval. *)
+(*     inversion Hval as [?? Hphi |ex' atr' c [? σ'] δ' iex' iatr' oζ ℓ Hphi [=] ? Hinf]; simplify_eq. *)
+(*     - inversion Hem; inversion Ham. econstructor; eauto. *)
+(*       pose proof (Hφ1 ex atr Hphi). *)
+(*       by simplify_eq. *)
+(*     - inversion Hem; inversion Ham. subst. *)
+(*       pose proof (valid_inf_system_trace_inv _ _ _ _ _ Hinf) as Hphi'. *)
+(*       specialize (Hφ2 (ex :tr[ oζ ]: (l, σ')) (atr :tr[ ℓ ]: δ') Hphi') as STEP. *)
+(*       red in STEP. *)
+(*       econstructor. *)
+(*       + eauto. *)
+(*       + eauto. *)
+(*       + match goal with *)
+(*         | [H: exec_trace_match _ iex' _ |- _] => inversion H; clear H; simplify_eq *)
+(*         end; done. *)
+(*       + match goal with *)
+(*         | [H: exec_trace_match _ iatr' _ |- _] => inversion H; clear H; simplify_eq *)
+(*         end; eapply STEP_EM; eauto. *)
+(*       + eapply IH; eauto. *)
+(*   Qed. *)
+
+(* End TracesMatch. *)
