fairness/heap_lang/execution_model.v
@@ -1,7 +1,0 @@
-From stdpp Require Import fin_maps.
-From iris.proofmode Require Import tactics.
-(* From trillium.program_logic Require Export weakestpre adequacy. *)
-(* From trillium.fairness Require Export fairness. *)
-From trillium.fairness.heap_lang Require Export lang.
-
-
